Update functions_order.rs

examples/functions/functions_order.rs
@@ -1,23 +1,67 @@
-pub struct SomeType(u32);
+pub struct SomeType(u32); // functions_order::SomeType
 
 impl SomeType {
-    pub fn meth1(self) { self.meth2(); }
-    fn meth2(self) {}
+    pub fn meth1(self) {
+        self.meth2();
+    } // functions_order::impl_SomeType::meth1
+    fn meth2(self) {} // functions_order::impl_SomeType::meth2
+}
+
+impl Default for SomeType {
+    fn default() -> SomeType {
+        SomeType(42)
+    }
 }
 
 mod inner_mod {
+    // functions_order::inner_mod
     pub fn bar() {
-	tar();
+        // functions_order::inner_mod::bar
+        tar();
     }
-    
-    fn tar() {}
+
+    fn tar() {} // functions_order::inner_mod::bar
+
+    mod nested_mod {
+        pub fn tick() {
+            tack();
+        }
+        fn tack() {}
+    }
 }
 
 fn main() {
+    // functions_order::main
     foo();
     inner_mod::bar();
     SomeType(0).meth1();
 }
 
-fn foo() {}
+fn foo() {} // functions_order::foo
 
+/*
+
+- type definitions
+- fucntion definitions
+- impl definitions
+- module definitions
+- impl trait definitions
+
+{
+  "reorder": {
+    "functions_order": {
+      "top_level": [
+         "SomeType",
+         "impl_SomeType",
+         "inner_mod",
+         "foo",
+         "main"
+      ],
+      "impl_Default_for_SomeType": ["default"]
+      "impl_SomeType": ["meth2", "meth1"]
+      "inner_mod": ["tar", "bar"],
+       inner_mod::nested_mod": ["tack", "tick"],
+    },
+  }
+}
+*/
