coq_translation/default/examples/functions/functions_order.v
@@ -33,12 +33,36 @@ Module Impl_functions_order_SomeType.
   }.
 End Impl_functions_order_SomeType.
 
+Module Impl_core_default_Default_for_functions_order_SomeType.
+  Definition Self := functions_order.SomeType.
+  
+  Definition default `{H : State.Trait} : M (H := H) functions_order.SomeType :=
+    Pure (functions_order.SomeType.Build_t 42).
+  
+  Global Instance AssociatedFunction_default `{H : State.Trait} :
+    Notation.DoubleColon Self "default" := {
+    Notation.double_colon := default;
+  }.
+  
+  Global Instance I : core.default.Default.Trait Self := {
+    core.default.Default.default `{H : State.Trait} := default;
+  }.
+End Impl_core_default_Default_for_functions_order_SomeType.
+
 Module inner_mod.
   Definition bar `{H : State.Trait} : M (H := H) unit :=
     let* _ := functions_order.inner_mod.tar in
     Pure tt.
   
   Definition tar `{H : State.Trait} : M (H := H) unit := Pure tt.
+  
+  Module nested_mod.
+    Definition tick `{H : State.Trait} : M (H := H) unit :=
+      let* _ := functions_order.inner_mod.nested_mod.tack in
+      Pure tt.
+    
+    Definition tack `{H : State.Trait} : M (H := H) unit := Pure tt.
+  End nested_mod.
 End inner_mod.
 
 Definition bar `{H : State.Trait} : M (H := H) unit :=
@@ -47,7 +71,19 @@ Definition bar `{H : State.Trait} : M (H := H) unit :=
 
 Definition tar `{H : State.Trait} : M (H := H) unit := Pure tt.
 
-Definition foo `{H : State.Trait} : M (H := H) unit := Pure tt.
+Module nested_mod.
+  Definition tick `{H : State.Trait} : M (H := H) unit :=
+    let* _ := functions_order.inner_mod.nested_mod.tack in
+    Pure tt.
+  
+  Definition tack `{H : State.Trait} : M (H := H) unit := Pure tt.
+End nested_mod.
+
+Definition tick `{H : State.Trait} : M (H := H) unit :=
+  let* _ := functions_order.inner_mod.nested_mod.tack in
+  Pure tt.
+
+Definition tack `{H : State.Trait} : M (H := H) unit := Pure tt.
 
 (* #[allow(dead_code)] - function was ignored by the compiler *)
 Definition main `{H : State.Trait} : M (H := H) unit :=
@@ -55,3 +91,5 @@ Definition main `{H : State.Trait} : M (H := H) unit :=
   let* _ := functions_order.inner_mod.bar in
   let* _ := (functions_order.SomeType.Build_t 0).["meth1"] in
   Pure tt.
+
+Definition foo `{H : State.Trait} : M (H := H) unit := Pure tt.
